exp_tsel_ind: simplify, eliminate varH

dev2019/dsubsup_total_rec_exp_tsel_ind.v
@@ -23,7 +23,6 @@ Definition id := nat.
 (* term variables occurring in types *)
 Inductive var : Type :=
 | varF : id -> var (* free, in concrete environment *)
-| varH : id -> var (* free, in abstract environment  *)
 | varB : id -> var (* locally-bound variable *)
 .
 
@@ -76,57 +75,54 @@ Fixpoint indexr {X : Type} (n : id) (l : list X) : option X :=
       if (beq_nat n (length l')) then Some a else indexr n l'
   end.
 
-Inductive closed: nat(*B*) -> nat(*H*) -> nat(*F*) -> ty -> Prop :=
-| cl_top: forall i j k,
-    closed i j k TTop
-| cl_bot: forall i j k,
-    closed i j k TBot
-| cl_all: forall i j k T1 T2,
-    closed i j k T1 ->
-    closed (S i) j k T2 ->
-    closed i j k (TAll T1 T2)
+Inductive closed: nat(*B*) -> nat(*F*) -> ty -> Prop :=
+| cl_top: forall i k,
+    closed i k TTop
+| cl_bot: forall i k,
+    closed i k TBot
+| cl_all: forall i k T1 T2,
+    closed i k T1 ->
+    closed (S i) k T2 ->
+    closed i k (TAll T1 T2)
 (* Now we have mutually recursive definitions for closedness on types and terms! *)
-| cl_sel_tm: forall i j k t,
-    closed_tm i j k t ->
-    closed i j k (TSel t)
-| cl_mem: forall i j k T1 T2,
-    closed i j k T1 ->
-    closed i j k T2 ->
-    closed i j k (TMem T1 T2)
-| cl_bind: forall i j k T,
-    closed (S i) j k T ->
-    closed i j k (TBind T)
-| cl_and: forall i j k T1 T2,
-    closed i j k T1 ->
-    closed i j k T2 ->
-    closed i j k (TAnd T1 T2)
+| cl_sel_tm: forall i k t,
+    closed_tm i k t ->
+    closed i k (TSel t)
+| cl_mem: forall i k T1 T2,
+    closed i k T1 ->
+    closed i k T2 ->
+    closed i k (TMem T1 T2)
+| cl_bind: forall i k T,
+    closed (S i) k T ->
+    closed i k (TBind T)
+| cl_and: forall i k T1 T2,
+    closed i k T1 ->
+    closed i k T2 ->
+    closed i k (TAnd T1 T2)
 
 
-with closed_tm: nat(*B*) -> nat(*H*) -> nat(*F*) -> tm -> Prop :=
-| cl_tvarb: forall i j k x,
+with closed_tm: nat(*B*) -> nat(*F*) -> tm -> Prop :=
+| cl_tvarb: forall i k x,
     i > x ->
-    closed_tm i j k (tvar (varB x))
-| cl_tvarh: forall i j k x,
-    j > x ->
-    closed_tm i j k (tvar (varH x))
-| cl_tvarf: forall i j k x,
+    closed_tm i k (tvar (varB x))
+| cl_tvarf: forall i k x,
     k > x ->
-    closed_tm i j k (tvar (varF x))
-| cl_ttyp:  forall i j k ty,
-    closed i j k ty ->
-    closed_tm i j k (ttyp ty)
-| cl_tabs:  forall i j k ty tm,
-    closed i j k ty ->
-    closed_tm (S i) j k tm ->
-    closed_tm i j k (tabs ty tm)
-| cl_tapp:  forall i j k tm1 tm2,
-    closed_tm i j k tm1 ->
-    closed_tm i j k tm2 ->
-    closed_tm i j k (tapp tm1 tm2)
-| cl_tunpack: forall i j k tm1 tm2,
-    closed_tm i j k tm1 ->
-    closed_tm (S i) j k tm2 ->
-    closed_tm i j k (tunpack tm1 tm2)
+    closed_tm i k (tvar (varF x))
+| cl_ttyp:  forall i k ty,
+    closed i k ty ->
+    closed_tm i k (ttyp ty)
+| cl_tabs:  forall i k ty tm,
+    closed i k ty ->
+    closed_tm (S i) k tm ->
+    closed_tm i k (tabs ty tm)
+| cl_tapp:  forall i k tm1 tm2,
+    closed_tm i k tm1 ->
+    closed_tm i k tm2 ->
+    closed_tm i k (tapp tm1 tm2)
+| cl_tunpack: forall i k tm1 tm2,
+    closed_tm i k tm1 ->
+    closed_tm (S i) k tm2 ->
+    closed_tm i k (tunpack tm1 tm2)
 .
 
 (* open define a locally-nameless encoding wrt to TVarB type variables. *)
@@ -137,9 +133,6 @@ Fixpoint open_rec (k: nat) (u: var) (T: ty) { struct T }: ty :=
     | TBot        => TBot
     | TAll T1 T2  => TAll (open_rec k u T1) (open_rec (S k) u T2)
     | TSel tm => TSel (open_rec_tm k u tm)
-    (* | TSel (tvar (varF x)) => TSel (tvar (varF x)) *)
-    (* | TSel (tvar (varH i)) => TSel (tvar (varH i)) *)
-    (* | TSel (tvar (varB i)) => if beq_nat k i then TSel (tvar u) else TSel (tvar (varB i)) *)
     | TMem T1 T2  => TMem (open_rec k u T1) (open_rec k u T2)
     | TBind T => TBind (open_rec (S k) u T)
     | TAnd T1 T2 => TAnd (open_rec k u T1) (open_rec k u T2)
@@ -148,7 +141,6 @@ Fixpoint open_rec (k: nat) (u: var) (T: ty) { struct T }: ty :=
 with open_rec_tm (k: nat) (u: var) (t: tm) { struct t }: tm :=
        match t with
        | tvar (varF x) => tvar (varF x)
-       | tvar (varH x) => tvar (varH x)
        | tvar (varB x) =>
          if beq_nat k x then (tvar u) else (tvar (varB x))
        | ttyp ty => ttyp (open_rec k u ty)
@@ -160,168 +152,133 @@ with open_rec_tm (k: nat) (u: var) (t: tm) { struct t }: tm :=
 Definition open u T := open_rec 0 u T.
 Definition open_tm u t := open_rec_tm 0 u t.
 
-(* Locally-nameless encoding with respect to varH variables. *)
-Fixpoint subst (U : var) (T : ty) {struct T} : ty :=
-  match T with
-    | TTop         => TTop
-    | TBot         => TBot
-    | TAll T1 T2   => TAll (subst U T1) (subst U T2)
-    | TSel t       => TSel (subst_tm U t)
-    | TMem T1 T2     => TMem (subst U T1) (subst U T2)
-    | TBind T       => TBind (subst U T)
-    | TAnd T1 T2    => TAnd (subst U T1)(subst U T2)
-  end
+(* (* Locally-nameless encoding with respect to varH variables. *) *)
+(* Fixpoint subst (U : var) (T : ty) {struct T} : ty := *)
+(*   match T with *)
+(*     | TTop         => TTop *)
+(*     | TBot         => TBot *)
+(*     | TAll T1 T2   => TAll (subst U T1) (subst U T2) *)
+(*     | TSel t       => TSel (subst_tm U t) *)
+(*     | TMem T1 T2     => TMem (subst U T1) (subst U T2) *)
+(*     | TBind T       => TBind (subst U T) *)
+(*     | TAnd T1 T2    => TAnd (subst U T1)(subst U T2) *)
+(*   end *)
 
-with subst_tm (U: var) (t: tm) {struct t} : tm :=
-       match t with
-       | tvar (varB i) => (tvar (varB i))
-       | tvar (varF i) => (tvar (varF i))
-       | tvar (varH i) => if beq_nat i 0 then tvar U else  (tvar (varH (i-1)))
-       | ttyp ty => ttyp (subst U ty)
-       | tabs ty tm => tabs (subst U ty) (subst_tm U tm)
-       | tapp tm1 tm2 => tapp (subst_tm U tm1) (subst_tm U tm2)
-       | tunpack tm1 tm2 => tunpack (subst_tm U tm1) (subst_tm U tm2)
-       end.
+(* with subst_tm (U: var) (t: tm) {struct t} : tm := *)
+(*        match t with *)
+(*        | tvar (varB i) => (tvar (varB i)) *)
+(*        | tvar (varF i) => (tvar (varF i)) *)
+(*        | tvar (varH i) => if beq_nat i 0 then tvar U else  (tvar (varH (i-1))) *)
+(*        | ttyp ty => ttyp (subst U ty) *)
+(*        | tabs ty tm => tabs (subst U ty) (subst_tm U tm) *)
+(*        | tapp tm1 tm2 => tapp (subst_tm U tm1) (subst_tm U tm2) *)
+(*        | tunpack tm1 tm2 => tunpack (subst_tm U tm1) (subst_tm U tm2) *)
+(*        end. *)
 
-Fixpoint nosubst (T : ty) {struct T} : Prop :=
-  match T with
-    | TTop         => True
-    | TBot         => True
-    | TAll T1 T2   => nosubst T1 /\ nosubst T2
-    (* | TSel (tvar (varB i)) => True *)
-    (* | TSel (tvar (varF i)) => True *)
-    (* | TSel (tvar (varH i)) => i <> 0 *)
-    | TSel t       => nosubst_tm t
-    | TMem T1 T2    => nosubst T1 /\ nosubst T2
-    | TBind T       => nosubst T
-    | TAnd T1 T2    => nosubst T1 /\ nosubst T2
-  end
+(* Fixpoint nosubst (T : ty) {struct T} : Prop := *)
+(*   match T with *)
+(*     | TTop         => True *)
+(*     | TBot         => True *)
+(*     | TAll T1 T2   => nosubst T1 /\ nosubst T2 *)
+(*     (* | TSel (tvar (varB i)) => True *) *)
+(*     (* | TSel (tvar (varF i)) => True *) *)
+(*     (* | TSel (tvar (varH i)) => i <> 0 *) *)
+(*     | TSel t       => nosubst_tm t *)
+(*     | TMem T1 T2    => nosubst T1 /\ nosubst T2 *)
+(*     | TBind T       => nosubst T *)
+(*     | TAnd T1 T2    => nosubst T1 /\ nosubst T2 *)
+(*   end *)
 
-with nosubst_tm (t: tm) {struct t} : Prop :=
-       match t with
-       | tvar (varB _) => True
-       | tvar (varF _) => True
-       | tvar (varH i) => i <> 0
-       | ttyp ty =>  nosubst ty
-       | tabs ty tm => (nosubst ty) /\ (nosubst_tm tm)
-       | tapp tm1 tm2 => (nosubst_tm tm1) /\ (nosubst_tm tm2)
-       | tunpack tm1 tm2 => (nosubst_tm tm1) /\ (nosubst_tm tm2)
-       end.
+(* with nosubst_tm (t: tm) {struct t} : Prop := *)
+(*        match t with *)
+(*        | tvar (varB _) => True *)
+(*        | tvar (varF _) => True *)
+(*        | tvar (varH i) => i <> 0 *)
+(*        | ttyp ty =>  nosubst ty *)
+(*        | tabs ty tm => (nosubst ty) /\ (nosubst_tm tm) *)
+(*        | tapp tm1 tm2 => (nosubst_tm tm1) /\ (nosubst_tm tm2) *)
+(*        | tunpack tm1 tm2 => (nosubst_tm tm1) /\ (nosubst_tm tm2) *)
+(*        end. *)
 
 (* ### Subtyping ### *)
-(*
-Note: In contrast to the rules on paper, the subtyping
-relation has two environments instead of just one.
-(The same holds for the semantic types, val_type, below).
-This split into an abstract and a concrete environment
-was necessary in the D<: soundness development, but is
-not required here. We just keep it for consistency with
-our earlier Coq files.
-
-The first env is for looking up varF variables.
-The first env matches the concrete runtime environment, and is
-extended during type assignment.
-The second env is for looking up varH variables.
-The second env matches the abstract runtime environment, and is
-extended during subtyping.
-*)
-Inductive stp: tenv -> tenv -> ty -> ty -> Prop :=
-| stp_top: forall G1 GH T1,
-    closed 0 (length GH) (length G1) T1 ->
-    stp G1 GH T1 TTop
-| stp_bot: forall G1 GH T2,
-    closed 0 (length GH) (length G1) T2 ->
-    stp G1 GH TBot T2
-| stp_mem: forall G1 GH S1 U1 S2 U2,
-    stp G1 GH U1 U2 ->
-    stp G1 GH S2 S1 ->
-    stp G1 GH (TMem S1 U1) (TMem S2 U2)
+Inductive stp: tenv -> ty -> ty -> Prop :=
+| stp_top: forall Gamma T1,
+    closed 0 (length Gamma) T1 ->
+    stp Gamma T1 TTop
+| stp_bot: forall Gamma T2,
+    closed 0 (length Gamma) T2 ->
+    stp Gamma TBot T2
+| stp_mem: forall Gamma S1 U1 S2 U2,
+    stp Gamma U1 U2 ->
+    stp Gamma S2 S1 ->
+    stp Gamma (TMem S1 U1) (TMem S2 U2)
 (* we move type selection into the typing relation has_type below *)
-(* | stp_sel1: forall G1 GH TX T2 tm, *)
-(*     has_type G1 tm TX -> *)
+(* | stp_sel1: forall Gamma GH TX T2 tm, *)
+(*     has_type Gamma tm TX -> *)
 (*     (* TODO: see if we can make the closedness conditions here and elsewhere *)
 (*        an invariant of has_type *) *)
-(*     closed 0 0 (length G1) TX -> *)
-(*     closed_tm 0 0 (length G1) tm -> *)
-(*     stp G1 GH TX (TMem TBot T2) -> *)
-(*     stp G1 GH (TSel tm) T2 *)
-(* | stp_sel2: forall G1 GH TX T1 tm, *)
-(*     has_type G1 tm TX -> *)
-(*     closed 0 0 (length G1) TX -> *)
-(*     closed_tm 0 0 (length G1) tm -> *)
-(*     stp G1 GH TX (TMem T1 TTop) -> *)
-(*     stp G1 GH T1 (TSel tm) *)
-| stp_selx: forall G1 GH tm, (*TODO rename the rule *)
-    (* this will also handle the stp_selax case from the previous version *)
-    closed_tm 0 (length GH) (length G1) tm ->
-    stp G1 GH (TSel tm) (TSel tm)
-
-(* TODO: it seems acceptable to adopt these from the previous version,
-since varH occurrences are artifacts of subtyping  *)
-| stp_sela1: forall G1 GH TX T2 x,
-    indexr x GH = Some TX ->
-    closed 0 x (length G1) TX ->
-    stp G1 GH TX (TMem TBot T2) ->
-    stp G1 GH (TSel (tvar (varH x))) T2
-| stp_sela2: forall G1 GH TX T1 x,
-    indexr x GH = Some TX ->
-    closed 0 x (length G1) TX ->
-    stp G1 GH TX (TMem T1 TTop) ->
-    stp G1 GH T1 (TSel (tvar (varH x)))
-
-(* this has become superfluous:   *)
-(* | stp_selax: forall G1 GH v x, *)
-(*     indexr x GH = Some v  -> *)
-(*     stp G1 GH (TSel (tvar (varH x))) (TSel (tvar (varH x))) *)
+(*     closed 0 0 (length Gamma) TX -> *)
+(*     closed_tm 0 0 (length Gamma) tm -> *)
+(*     stp Gamma GH TX (TMem TBot T2) -> *)
+(*     stp Gamma GH (TSel tm) T2 *)
+(* | stp_sel2: forall Gamma GH TX T1 tm, *)
+(*     has_type Gamma tm TX -> *)
+(*     closed 0 0 (length Gamma) TX -> *)
+(*     closed_tm 0 0 (length Gamma) tm -> *)
+(*     stp Gamma GH TX (TMem T1 TTop) -> *)
+(*     stp Gamma GH T1 (TSel tm) *)
+| stp_sel: forall Gamma tm,
+    closed_tm 0 (length Gamma) tm ->
+    stp Gamma (TSel tm) (TSel tm)
 
 (* stp for recursive types and intersection types *)
-| stp_bindx: forall GH G1 T1 T1' T2 T2',
-    stp G1 (T1'::GH) T1' T2' ->
-    T1' = (open (varH (length GH)) T1) ->
-    T2' = (open (varH (length GH)) T2) ->
-    closed 1 (length GH) (length G1) T1 ->
-    closed 1 (length GH) (length G1) T2 ->
-    stp G1 GH (TBind T1) (TBind T2)
+| stp_bindx: forall  Gamma T1 T1' T2 T2',
+    stp (T1'::Gamma) T1' T2' ->
+    T1' = (open (varF (length Gamma)) T1) ->
+    T2' = (open (varF (length Gamma)) T2) ->
+    closed 1 (length Gamma) T1 ->
+    closed 1 (length Gamma) T2 ->
+    stp Gamma (TBind T1) (TBind T2)
 
-| stp_and11: forall GH G1 T1 T2 T,
-    stp G1 GH T1 T ->
-    closed 0 (length GH) (length G1) T2 ->
-    stp G1 GH (TAnd T1 T2) T
+| stp_and11: forall Gamma T1 T2 T,
+    stp Gamma T1 T ->
+    closed 0 (length Gamma) T2 ->
+    stp Gamma (TAnd T1 T2) T
 
-| stp_and12: forall GH G1 T1 T2 T,
-    stp G1 GH T2 T ->
-    closed 0 (length GH) (length G1) T1 ->
-    stp G1 GH (TAnd T1 T2) T
+| stp_and12: forall Gamma T1 T2 T,
+    stp Gamma T2 T ->
+    closed 0 (length Gamma) T1 ->
+    stp Gamma (TAnd T1 T2) T
 
-| stp_and2: forall GH G1 T1 T2 T,
-    stp G1 GH T T1 ->
-    stp G1 GH T T2 ->
-    stp G1 GH T (TAnd T1 T2)
+| stp_and2: forall Gamma T1 T2 T,
+    stp Gamma T T1 ->
+    stp Gamma T T2 ->
+    stp Gamma T (TAnd T1 T2)
 
-| stp_all: forall G1 GH T1 T2 T3 T4 x,
-    stp G1 GH T3 T1 ->
-    x = length GH ->
-    closed 1 (length GH) (length G1) T2 ->
-    closed 1 (length GH) (length G1) T4 ->
-    stp G1 (T3::GH) (open (varH x) T2) (open (varH x) T4) ->
-    stp G1 GH (TAll T1 T2) (TAll T3 T4)
+| stp_all: forall Gamma T1 T2 T3 T4 x,
+    stp Gamma T3 T1 ->
+    x = length Gamma ->
+    closed 1 (length Gamma) T2 ->
+    closed 1 (length Gamma) T4 ->
+    stp (T3::Gamma) (open (varF x) T2) (open (varF x) T4) ->
+    stp Gamma (TAll T1 T2) (TAll T3 T4)
 
-| stp_trans: forall G1 GH T1 T2 T3,
-    stp G1 GH T1 T2 ->
-    stp G1 GH T2 T3 ->
-    stp G1 GH T1 T3
+| stp_trans: forall Gamma T1 T2 T3,
+    stp Gamma T1 T2 ->
+    stp Gamma T2 T3 ->
+    stp Gamma T1 T3
 
 (* ### Type Assignment ### *)
 with has_type : tenv -> tm -> ty -> Prop :=
-| t_var: forall x env T1,
-           indexr x env = Some T1 ->
-           stp env [] T1 T1 ->
-           has_type env (tvar (varF x)) T1
+| t_var: forall x Gamma T1,
+           indexr x Gamma = Some T1 ->
+           stp Gamma T1 T1 -> (* TODO necessary? *)
+           has_type Gamma (tvar (varF x)) T1
 (* pack a recursive type  *)
-| t_var_pack : forall G1 x T1,
-           has_type G1 (tvar x) (open x T1) ->
-           closed 1 0 (length G1) T1 ->
-           has_type G1 (tvar x) (TBind T1)
+| t_var_pack : forall Gamma x T1,
+           has_type Gamma (tvar x) (open x T1) ->
+           closed 1 (length Gamma) T1 ->
+           has_type Gamma (tvar x) (TBind T1)
 
            (* (* has_type G1 (tvar x) T1' -> *) *)
            (* indexr x G1 = Some (open (varF x) T1) -> *)
@@ -329,52 +286,52 @@ with has_type : tenv -> tm -> ty -> Prop :=
            (* closed 1 0 (length G1) T1 -> *)
            (* has_type G1 (tvar (varF x)) (TBind T1) *)
 (* unpack a recursive type: unpack(x:{z=>T^z}) { x:T^x => ... }  *)
-| t_unpack: forall env x y T1 T1' T2,
-           has_type env x (TBind T1) ->
-           T1' = (open (varF (length env)) T1) ->
-           has_type (T1'::env) y T2 ->
-           closed 0 0 (length env) T2 ->
-           has_type env (tunpack x y) T2
+| t_unpack: forall Gamma x y T1 T1' T2,
+           has_type Gamma x (TBind T1) ->
+           T1' = (open (varF (length Gamma)) T1) ->
+           has_type (T1'::Gamma) y T2 ->
+           closed 0 (length Gamma) T2 ->
+           has_type Gamma (tunpack x y) T2
 
 (* intersection typing *)
-| t_and : forall env x T1 T2,
-           has_type env (tvar x) T1 ->
-           has_type env (tvar x) T2 ->
-           has_type env (tvar x) (TAnd T1 T2)
+| t_and : forall Gamma x T1 T2,
+           has_type Gamma (tvar x) T1 ->
+           has_type Gamma (tvar x) T2 ->
+           has_type Gamma (tvar x) (TAnd T1 T2)
 
 
-| t_typ: forall env T1,
-           closed 0 0 (length env) T1 ->
-           has_type env (ttyp T1) (TMem T1 T1)
+| t_typ: forall Gamma T1,
+           closed 0 (length Gamma) T1 ->
+           has_type Gamma (ttyp T1) (TMem T1 T1)
 
-| t_app: forall env f x T1 T2,
-           has_type env f (TAll T1 T2) ->
-           has_type env x T1 ->
-           closed 0 0 (length env) T2 ->
-           has_type env (tapp f x) T2
-| t_dapp: forall env f x T1 T2 T,
-           has_type env f (TAll T1 T2) ->
-           has_type env (tvar (varF x)) T1 ->
+| t_app: forall Gamma f x T1 T2,
+           has_type Gamma f (TAll T1 T2) ->
+           has_type Gamma x T1 ->
+           closed 0 (length Gamma) T2 ->
+           has_type Gamma (tapp f x) T2
+| t_dapp: forall Gamma f x T1 T2 T,
+           has_type Gamma f (TAll T1 T2) ->
+           has_type Gamma (tvar (varF x)) T1 ->
            T = open (varF x) T2 ->
-           closed 0 0 (length env) T ->
-           has_type env (tapp f (tvar (varF x))) T
-| t_abs: forall env y T1 T2,
-           has_type (T1::env) y (open (varF (length env)) T2) ->
-           closed 0 0 (length env) (TAll T1 T2) ->
-           has_type env (tabs T1 y) (TAll T1 T2)
-| t_sub: forall env e T1 T2,
-           has_type env e T1 ->
-           stp env [] T1 T2 ->
-           has_type env e T2
+           closed 0 (length Gamma) T ->
+           has_type Gamma (tapp f (tvar (varF x))) T
+| t_abs: forall Gamma y T1 T2,
+           has_type (T1::Gamma) y (open (varF (length Gamma)) T2) ->
+           closed 0 (length Gamma) (TAll T1 T2) ->
+           has_type Gamma (tabs T1 y) (TAll T1 T2)
+| t_sub: forall Gamma e T1 T2,
+           has_type Gamma e T1 ->
+           stp Gamma T1 T2 ->
+           has_type Gamma e T2
 
-| t_sel_intro: forall env e1 e2 T,
-    has_type env e1 T ->
-    has_type env e2 (TMem T TTop) ->
-    has_type env e1 (TSel e2)
-| t_sel_elim: forall env e1 e2 T,
-    has_type env e1 (TSel e2) ->
-    has_type env e2 (TMem TBot T) ->
-    has_type env e1 T
+| t_sel_intro: forall Gamma e1 e2 T,
+    has_type Gamma e1 T ->
+    has_type Gamma e2 (TMem T TTop) ->
+    has_type Gamma e1 (TSel e2)
+| t_sel_elim: forall Gamma e1 e2 T,
+    has_type Gamma e1 (TSel e2) ->
+    has_type Gamma e2 (TMem TBot T) ->
+    has_type Gamma e1 T
 .
 
 
@@ -399,7 +356,6 @@ Fixpoint teval(n: nat)(env: venv)(t: tm){struct n}: option (option vl) :=
     | S n =>
       match t with
         | tvar (varF x) => Some (indexr x env)
-        | tvar (varH x) => Some None
         | tvar (varB x) => Some None
         | ttyp T       => Some (Some (vty env T)) (* TODO: should T be normalized? *)
         | tabs T y     => Some (Some (vabs env T y)) (* TODO: should T be normalized? *)
@@ -461,63 +417,68 @@ Definition vset_sub_eq {n:nat}: vset n -> vset n -> Prop :=
 Definition vseta_sub_eq (vs1: vseta) (vs2: vseta) :=
   forall n, vset_sub_eq (vs1 n) (vs2 n).
 
+Definition renv := list vseta.
+
 (* Requires no termination proof and is invertible *)
-Inductive logrel_ty: list vseta -> list vseta -> ty -> forall n, vset n -> vl -> Prop :=
-| LTop: forall Gamma GH n vsn v, logrel_ty Gamma GH TTop n vsn v
-| LTMem: forall Gamma GH n T1 vsn1 T2 vsn2 vl1 vl2 H Tx vsn,
-    logrel_ty Gamma GH T1 n vsn1 vl1 ->
-    logrel_ty Gamma GH T2 n vsn2 vl2 ->
+Inductive logrel_ty: renv  -> ty -> forall n, vset n -> vl -> Prop :=
+| LTop: forall rho n vsn v,
+    logrel_ty rho TTop n vsn v
+
+| LTMem: forall rho n T1 vsn1 T2 vsn2 vl1 vl2 H Tx vsn,
+    logrel_ty rho T1 n vsn1 vl1 ->
+    logrel_ty rho T2 n vsn2 vl2 ->
     vset_sub_eq vsn1 vsn ->
     vset_sub_eq vsn vsn2 ->
-    logrel_ty Gamma GH (TMem T1 T2) n vsn (vty H Tx)
-| LTAll: forall Gamma GH n T1 T2 vsn1 vl1 vsn H T0 t,
-    logrel_ty Gamma GH T1 n vsn1 vl1 ->
+    logrel_ty rho (TMem T1 T2) n vsn (vty H Tx)
+
+| LTAll: forall rho n T1 T2 vsn1 vl1 vsn H T0 t,
+    logrel_ty rho T1 n vsn1 vl1 ->
     (exists (vs2 : vseta) vl2,
       tevaln (vl1 :: H) t vl2
-       /\ forall k, logrel_ty Gamma (vs2 :: GH) (open (varH (length Gamma)) T2) k (vs2 k) vl2) ->
-    logrel_ty Gamma GH (TAll T1 T2) n vsn (vabs H T0 t)
-| LTSel: forall Gamma GH n t vsn v,
-    logrel_tm Gamma GH t n vsn v ->
-    logrel_ty Gamma GH (TSel t) n vsn v
-| LTAnd: forall Gamma GH n T1 T2 vsn v,
-    logrel_ty Gamma GH T1 n vsn v ->
-    logrel_ty Gamma GH T2 n vsn v ->
-    logrel_ty Gamma GH (TAnd T1 T2) n vsn v
-| LTBind: forall Gamma GH n T vsn v,
+      /\ forall k, logrel_ty (vs2 :: rho) (open (varF (length rho)) T2) k (vs2 k) vl2) ->
+    logrel_ty rho (TAll T1 T2) n vsn (vabs H T0 t)
+
+| LTSel: forall rho n t vsn v,
+    logrel_tm rho t n vsn v ->
+    logrel_ty rho (TSel t) n vsn v
+
+| LTAnd: forall rho n T1 T2 vsn v,
+    logrel_ty rho T1 n vsn v ->
+    logrel_ty rho T2 n vsn v ->
+    logrel_ty rho (TAnd T1 T2) n vsn v
+
+| LTBind: forall rho n T vsn v,
     (exists (vs: vseta),
         (vs n) = vsn
-        /\ forall k, logrel_ty Gamma (vs :: GH) (open (varH (length GH)) T) k (vs k) v) ->
-    logrel_ty Gamma GH (TBind T) n vsn v
+        /\ forall k, logrel_ty (vs :: rho) (open (varF (length rho)) T) k (vs k) v) ->
+    logrel_ty rho (TBind T) n vsn v
 
-with logrel_tm: list vseta -> list vseta -> tm -> forall n, vset n -> vl -> Prop :=
-| LVarF: forall Gamma GH n x (vs: vseta) vsn v,
-    (indexr x Gamma) = Some vs ->
+with logrel_tm: list vseta -> tm -> forall n, vset n -> vl -> Prop :=
+| LVarF: forall rho n x (vs: vseta) vsn v,
+    (indexr x rho) = Some vs ->
     vs (S n) vsn v ->
-    logrel_tm Gamma GH (tvar (varF x)) n vsn v
-| LVarH: forall Gamma GH n x (vs: vseta) vsn v,
-    (indexr x GH) = Some vs ->
-    vs (S n) vsn v ->
-    logrel_tm Gamma GH (tvar (varH x)) n vsn v
-| LTTyp: forall Gamma GH n T vsn v,
-    logrel_ty Gamma GH T n vsn v ->
-    logrel_tm Gamma GH (ttyp T) n vsn v
+    logrel_tm rho (tvar (varF x)) n vsn v
+
+| LTTyp: forall rho n T vsn v,
+    logrel_ty rho T n vsn v ->
+    logrel_tm rho (ttyp T) n vsn v
 .
 
-
 (* consistent environment *)
-Definition R_env venv genv tenv :=
-  length venv = length tenv /\
-  length genv = length tenv /\
-  forall x TX, indexr x tenv = Some TX ->
-    (exists (jj:vseta) vx,
+Definition R_env venv rho Gamma :=
+  length venv = length Gamma /\
+  length rho = length Gamma /\
+  forall x TX, indexr x Gamma = Some TX ->
+    (exists (vsx:vseta) vx,
        indexr x venv = Some vx /\
-       indexr x genv = Some jj /\
-       forall n, logrel_ty genv [] TX n (jj n) vx).
+       indexr x rho = Some vsx /\
+       forall n, logrel_ty rho TX n (vsx n) vx).
 
 
 (* automation *)
 Hint Unfold venv.
 Hint Unfold tenv.
+Hint Unfold renv.
 
 Hint Unfold open.
 Hint Unfold indexr.
@@ -539,10 +500,14 @@ Hint Constructors list.
 
 Hint Resolve ex_intro.
 
+Ltac ev := repeat match goal with
+                    | H: exists _, _ |- _ => destruct H
+                    | H: _ /\  _ |- _ => destruct H
+           end.
 
-Theorem full_total_safety : forall e tenv T,
-  has_type tenv e T -> forall venv renv, R_env venv renv tenv ->
-  exists (d: vseta) v, tevaln venv e v /\ forall k, logrel_ty renv [] T k (d k) v.
+Theorem full_total_safety : forall e Gamma T,
+  has_type Gamma e T -> forall venv rho, R_env venv rho Gamma ->
+  exists (d: vseta) v, tevaln venv e v /\ forall k, logrel_ty rho T k (d k) v.
 Proof.
   intros ? ? ? W.
   induction W; intros ? ? WFE.
@@ -560,9 +525,6 @@ Proof.
     assert (Wit := WFE).
     apply IHW in Wit.
     destruct Wit as [d0 [v0 [? ?]]].
-    unfold R_env in WFE. destruct WFE as [Hlen1 [Hlen2  Hlookup]].
+    unfold R_env in WFE. ev.
     exists d0. exists v0.
-    split.
-    auto.
-    intros k.
     Admitted.
